theories/terms.v
@@ -7,72 +7,79 @@ From stdpp Require Import prelude base gmap functions.
 (** * Bunched terms *)
 Inductive bterm (var : Type) : Type :=
 | Var (x : var)
-| TComma (T1 T2 : bterm var)
-| TSemic (T1 T2 : bterm var)
+| TBin (sp : sep) (T1 T2 : bterm var)
 .
 Arguments Var {_} x.
-Arguments TComma {_} T1 T2.
-Arguments TSemic {_} T1 T2.
+Arguments TBin {_} sp T1 T2.
 
-Global Instance bterm_eqdecision `{EqDecision A} : EqDecision (bterm A).
+#[export] Instance sep_eqdecision : EqDecision sep.
+Proof. solve_decision. Defined.
+#[export] Instance sep_countable : Countable sep.
+Proof.
+  set (enc := λ s, match s with Comma => 0 | SemiC => 1 end).
+  set (dec := λ n, match n with 0 => Comma | S _ => SemiC end).
+  apply (inj_countable' enc dec).
+  abstract (destruct x; simpl; eauto).
+Defined.
+
+#[export] Instance bterm_eqdecision `{EqDecision A} : EqDecision (bterm A).
 Proof. solve_decision. Qed.
+
 Global Instance bterm_countable : Countable (bterm nat).
 Proof.
  set (enc :=
-   fix go T :=
+   fix go T : gen_tree nat :=
      match T with
      | Var x => (GenLeaf x : gen_tree nat)
-     | TComma T1 T2 => GenNode 0 [go T1; go T2]
-     | TSemic T1 T2 => GenNode 1 [go T1; go T2]
+     | TBin sp T1 T2 => GenNode (Pos.to_nat (encode sp)) [go T1; go T2]
      end).
  set (dec :=
    fix go e :=
      match (e : gen_tree nat) with
      | GenLeaf x => Var x
-     | GenNode 0 [e1; e2] => TComma (go e1) (go e2)
-     | GenNode 1 [e1; e2] => TSemic (go e1) (go e2)
+     | GenNode i [e1; e2] =>
+         match (decode (Pos.of_nat i) : option sep) with
+         | Some sp => TBin sp (go e1) (go e2)
+         | None    => Var 0
+         end
      | _ => Var 0
      end).
  apply (inj_countable' enc dec).
- induction x; simpl; eauto; by rewrite IHx1 IHx2.
+ abstract (induction x; simpl; eauto;
+             by rewrite Pos2Nat.id decode_encode IHx1 IHx2).
 Defined.
 
 Fixpoint bterm_alg_act {PROP : bi} `{!EqDecision V,!Countable V}
          (T : bterm V) (Xs : V → PROP) : PROP :=
   match T with
   | Var v => Xs v
-  | TComma T1 T2 => bterm_alg_act T1 Xs ∗ bterm_alg_act T2 Xs
-  | TSemic T1 T2 => bterm_alg_act T1 Xs ∧ bterm_alg_act T2 Xs
+  | TBin sp T1 T2 => sep_interp sp (bterm_alg_act T1 Xs) (bterm_alg_act T2 Xs)
   end%I.
 
-Fixpoint bterm_ctx_act `{!EqDecision V,!Countable V}
-         (T : bterm V) (Δs : V → bunch) : bunch :=
+Fixpoint bterm_ctx_act {frml} `{!EqDecision V,!Countable V}
+         (T : bterm V) (Δs : V → @bunch frml) : @bunch frml :=
   match T with
   | Var v => Δs v
-  | TComma T1 T2 => bterm_ctx_act T1 Δs,, bterm_ctx_act T2 Δs
-  | TSemic T1 T2 => bterm_ctx_act T1 Δs;, bterm_ctx_act T2 Δs
+  | TBin sp T1 T2 => bbin sp (bterm_ctx_act T1 Δs) (bterm_ctx_act T2 Δs)
   end%B.
 
 Global Instance bterm_fmap : FMap bterm :=
   fix go _ _ f T { struct T } := let _ : FMap _ := go in
   match T with
   | Var x => Var (f x)
-  | TComma T1 T2 => TComma (f <$> T1) (f <$> T2)
-  | TSemic T1 T2 => TSemic (f <$> T1) (f <$> T2)
+  | TBin sp T1 T2 => TBin sp (f <$> T1) (f <$> T2)
   end.
 
 Fixpoint term_fv `{!EqDecision V,!Countable V} (T : bterm V) : gset V :=
   match T with
   | Var x => {[ x ]}
-  | TComma T1 T2 => term_fv T1 ∪ term_fv T2
-  | TSemic T1 T2 => term_fv T1 ∪ term_fv T2
+  | TBin sp T1 T2 => term_fv T1 ∪ term_fv T2
   end.
 
 Fixpoint linear_bterm `{!EqDecision V,!Countable V} (T : bterm V) : Prop :=
   match T with
   | Var x => True
-  | TComma T1 T2
-  | TSemic T1 T2 =>
+  | TBin sp T1 T2 =>
     term_fv T1 ## term_fv T2 ∧
     linear_bterm T1 ∧ linear_bterm T2
   end.
@@ -90,14 +97,10 @@ Fixpoint linear_bterm `{!EqDecision V,!Countable V} (T : bterm V) : Prop :=
 Fixpoint linearize_pre (T : bterm nat) (idx : nat) : nat * gmap nat nat * bterm nat :=
   match T with
   | Var x => (idx + 1, {[ idx := x ]}, Var idx)
-  | TComma T1 T2 =>
+  | TBin sp T1 T2 =>
       let '(idx1,m1,T1') := linearize_pre T1 idx in
       let '(idx2,m2,T2') := linearize_pre T2 idx1 in
-      (idx2, m1 ∪ m2, TComma T1' T2')
-  | TSemic T1 T2 =>
-      let '(idx1,m1,T1') := linearize_pre T1 idx in
-      let '(idx2,m2,T2') := linearize_pre T2 idx1 in
-      (idx2, m1 ∪ m2, TSemic T1' T2')
+      (idx2, m1 ∪ m2, TBin sp T1' T2')
   end.
 
 Definition linearize_bterm (T : bterm nat) : bterm nat := snd (linearize_pre T 0).
@@ -107,17 +110,14 @@ Definition linearize_bterm_ren (T : bterm nat) : gmap nat nat := snd $ fst (line
 Fixpoint bterm_gset_fold (T : bterm (gset nat)) : gset (bterm nat) :=
   match T with
   | Var X => set_map Var X
-  | TComma T1 T2 =>
+  | TBin sp T1 T2 =>
       let S1 := bterm_gset_fold T1 in
       let S2 := bterm_gset_fold T2 in
-      set_map_2 TComma S1 S2
-  | TSemic T1 T2 =>
-      let S1 := bterm_gset_fold T1 in
-      let S2 := bterm_gset_fold T2 in
-      set_map_2 TSemic S1 S2
+      set_map_2 (TBin sp) S1 S2
   end.
 
-Definition bterm_gset_fmap (f : nat → nat) (T : bterm (gset nat)) : bterm (gset nat) := set_map f <$> T.
+Definition bterm_gset_fmap (f : nat → nat) (T : bterm (gset nat)) : bterm (gset nat)
+  := set_map f <$> T.
 
 (** ** Structural rules *)
 
@@ -140,28 +140,23 @@ Proof.
   - f_equiv/=.
     + apply IHt1_1. set_solver.
     + apply IHt1_2. set_solver.
-  - f_equiv/=.
-    + apply IHt1_1. set_solver.
-    + apply IHt1_2. set_solver.
 Qed.
 
 Lemma bterm_fmap_compose {A B C} (f : A → B) (g : B → C) (T : bterm A) :
   (g ∘ f) <$> T = g <$> (f <$> T).
 Proof.
   induction T; simpl; auto.
-  - rewrite IHT1 IHT2 //.
-  - rewrite IHT1 IHT2 //.
+  rewrite IHT1 IHT2 //.
 Qed.
 
 (** ** interpretation properties *)
-Lemma bterm_ctx_act_fv `{!EqDecision V,!Countable V} (T : bterm V) Δs Γs :
+Lemma bterm_ctx_act_fv {frml} `{!EqDecision V,!Countable V} (T : bterm V)
+  (Δs Γs : V → @bunch frml) :
   (∀ i : V, i ∈ term_fv T → Δs i = Γs i) →
   bterm_ctx_act T Δs = bterm_ctx_act T Γs.
 Proof.
   induction T; simpl.
   - set_solver.
-  - set_unfold. intros H.
-    rewrite IHT1; eauto. rewrite IHT2; eauto.
   - set_unfold. intros H.
     rewrite IHT1; eauto. rewrite IHT2; eauto.
 Qed.
@@ -173,9 +168,7 @@ Proof.
   induction T; simpl.
   - set_solver.
   - set_unfold. intros H.
-    rewrite IHT1; eauto. rewrite IHT2; eauto.
-  - set_unfold. intros H.
-    rewrite IHT1; eauto. rewrite IHT2; eauto.
+    rewrite IHT1; eauto; rewrite IHT2; eauto.
 Qed.
 
 Lemma bterm_alg_act_mono {PROP : bi} `{!EqDecision V, !Countable V}
@@ -184,7 +177,7 @@ Lemma bterm_alg_act_mono {PROP : bi} `{!EqDecision V, !Countable V}
   bterm_alg_act T Xs ⊢ bterm_alg_act (PROP:=PROP) T Ys.
 Proof.
   intros HXY. induction T; simpl; auto.
-  all: by rewrite IHT1 IHT2.
+  by rewrite IHT1 IHT2.
 Qed.
 
 Lemma bterm_alg_act_mono' {PROP : bi} `{!EqDecision V, !Countable V}
@@ -194,12 +187,7 @@ Lemma bterm_alg_act_mono' {PROP : bi} `{!EqDecision V, !Countable V}
 Proof.
   intros HXY. induction T; simpl; eauto.
   - apply HXY. set_solver.
-  - f_equiv.
-    + apply IHT1. set_solver.
-    + apply IHT2. set_solver.
-  - f_equiv.
-    + apply IHT1. set_solver.
-    + apply IHT2. set_solver.
+  - f_equiv; first [apply IHT1 | apply IHT2]; set_solver.
 Qed.
 
 (** Interpretation of bunches is a homomorphism w.r.t. bunched terms:
@@ -214,13 +202,13 @@ Lemma bterm_ctx_alg_act {PROP : bi} `{!EqDecision V,!Countable V}
 Proof.
   induction T; simpl.
   - reflexivity.
-  - by rewrite IHT1 IHT2.
-  - by rewrite IHT1 IHT2.
+  - simpl; by rewrite IHT1 IHT2.
 Qed.
 
 (** Linear bunched terms can be viewed as _bunches with holes_, when
 restricted to one free variable. *)
-Lemma blinterm_ctx_act_insert `{!EqDecision V, !Countable V} (T : bterm V) Δs i :
+Lemma blinterm_ctx_act_insert {frml} `{!EqDecision V, !Countable V}
+  (T : bterm V) (Δs : V → @bunch frml) i :
   linear_bterm T →
   i ∈ term_fv T →
   ∃ (Π : bunch_ctx), ∀ Γ , fill Π Γ = bterm_ctx_act T (<[i:=Γ]>Δs).
@@ -232,7 +220,7 @@ Proof.
     set_unfold.
     destruct Hi as [Hi1 | Hi2].
     + destruct (IHT1 i Hlin1 Hi1) as (Π₁ & HΠ1).
-      exists (Π₁++[CtxCommaL (bterm_ctx_act T2 Δs)]).
+      exists (Π₁++[CtxL sp (bterm_ctx_act T2 Δs)]).
       intros Γ. rewrite fill_app /=.
       rewrite HΠ1. f_equiv.
       assert (i ∉ term_fv T2).
@@ -242,30 +230,7 @@ Proof.
       { naive_solver. }
       rewrite functions.fn_lookup_insert_ne//.
     + destruct (IHT2 i Hlin2 Hi2) as (Π₁ & HΠ1).
-      exists (Π₁++[CtxCommaR (bterm_ctx_act T1 Δs)]).
-      intros Γ. rewrite fill_app /=.
-      rewrite HΠ1. f_equiv.
-      assert (i ∉ term_fv T1).
-      { set_solver. }
-      apply bterm_ctx_act_fv.
-      intros j. destruct (decide (i = j)) as [->|?].
-      { naive_solver. }
-      rewrite functions.fn_lookup_insert_ne//.
-  - destruct Hlin as (Hdisj & Hlin1 & Hlin2).
-    set_unfold.
-    destruct Hi as [Hi1 | Hi2].
-    + destruct (IHT1 i Hlin1 Hi1) as (Π₁ & HΠ1).
-      exists (Π₁++[CtxSemicL (bterm_ctx_act T2 Δs)]).
-      intros Γ. rewrite fill_app /=.
-      rewrite HΠ1. f_equiv.
-      assert (i ∉ term_fv T2).
-      { set_solver. }
-      apply bterm_ctx_act_fv.
-      intros j. destruct (decide (i = j)) as [->|?].
-      { naive_solver. }
-      rewrite functions.fn_lookup_insert_ne//.
-    + destruct (IHT2 i Hlin2 Hi2) as (Π₁ & HΠ1).
-      exists (Π₁++[CtxSemicR (bterm_ctx_act T1 Δs)]).
+      exists (Π₁++[CtxR sp (bterm_ctx_act T1 Δs)]).
       intros Γ. rewrite fill_app /=.
       rewrite HΠ1. f_equiv.
       assert (i ∉ term_fv T1).
@@ -282,12 +247,6 @@ Lemma linearize_pre_mono T (idx1 : nat):
 Proof.
   revert idx1; induction T=>idx1 /=.
   - lia.
-  - specialize (IHT1 idx1).
-    destruct (linearize_pre T1 idx1) as [[i1 m1] T1'] eqn:Ht1.
-    specialize (IHT2 i1).
-    destruct (linearize_pre T2 i1) as [[idx2 m2] T2'] eqn:Ht2.
-
-    simpl in *. lia.
   - specialize (IHT1 idx1).
     destruct (linearize_pre T1 idx1) as [[i1 m1] T1'] eqn:Ht1.
     specialize (IHT2 i1).
@@ -313,17 +272,6 @@ Proof.
     { replace idx2 with (fst $ fst $ linearize_pre T2 i1); [ | by rewrite Ht2 ].
       apply linearize_pre_mono. }
     simpl. set_solver by lia.
-  - specialize (IHT1 idx1).
-    destruct (linearize_pre T1 idx1) as [[i1 m1] T1'] eqn:Ht1.
-    assert (idx1 ≤ i1).
-    { replace i1 with (fst $ fst $ linearize_pre T1 idx1); [ | by rewrite Ht1 ].
-      apply linearize_pre_mono. }
-    specialize (IHT2 i1).
-    destruct (linearize_pre T2 i1) as [[idx2 m2] T2'] eqn:Ht2.
-    assert (i1 ≤ idx2).
-    { replace idx2 with (fst $ fst $ linearize_pre T2 i1); [ | by rewrite Ht2 ].
-      apply linearize_pre_mono. }
-    simpl. set_solver by lia.
 Qed.
 
 Lemma linearize_pre_dom T (idx1 : nat):
@@ -333,19 +281,6 @@ Lemma linearize_pre_dom T (idx1 : nat):
 Proof.
   revert idx1; induction T=>idx1 /=.
   - set_unfold; lia.
-  - specialize (IHT1 idx1).
-    destruct (linearize_pre T1 idx1) as [[i1 m1] T1'] eqn:Ht1.
-    assert (idx1 ≤ i1).
-    { replace i1 with (fst $ fst $ linearize_pre T1 idx1); [ | by rewrite Ht1 ].
-      apply linearize_pre_mono. }
-    specialize (IHT2 i1).
-    destruct (linearize_pre T2 i1) as [[idx2 m2] T2'] eqn:Ht2.
-    assert (i1 ≤ idx2).
-    { replace idx2 with (fst $ fst $ linearize_pre T2 i1); [ | by rewrite Ht2 ].
-      apply linearize_pre_mono. }
-    simpl in *.
-    rewrite dom_union_L IHT1 IHT2.
-    set_solver by lia.
   - specialize (IHT1 idx1).
     destruct (linearize_pre T1 idx1) as [[i1 m1] T1'] eqn:Ht1.
     assert (idx1 ≤ i1).
@@ -380,20 +315,6 @@ Proof.
       replace idx2 with (fst $ fst (linearize_pre T2 i)) by rewrite Ht2 //.
       apply linearize_pre_fv. }
     set_solver by lia.
-  - specialize (IHT1 idx).
-    destruct (linearize_pre T1 idx) as [[i m1] T1'] eqn:Ht1.
-    specialize (IHT2 i).
-    destruct (linearize_pre T2 i) as [[idx2 m2] T2'] eqn:Ht2.
-    simpl. repeat split; eauto.
-    assert (term_fv T1' ⊆ set_seq idx (i-idx)).
-    { replace T1' with (snd (linearize_pre T1 idx)) by rewrite Ht1 //.
-      replace i with (fst $ fst (linearize_pre T1 idx)) by rewrite Ht1 //.
-      apply linearize_pre_fv. }
-    assert (term_fv T2' ⊆ set_seq i (idx2-i)).
-    { replace T2' with (snd (linearize_pre T2 i)) by rewrite Ht2 //.
-      replace idx2 with (fst $ fst (linearize_pre T2 i)) by rewrite Ht2 //.
-      apply linearize_pre_fv. }
-    set_solver by lia.
 Qed.
 
 (** ** term folding properties *)
@@ -404,28 +325,8 @@ Lemma bterm_gset_fold_fmap_inv (f : nat → gset nat) (T T' : bterm nat) :
   linear_bterm T →
   T' ∈ bterm_gset_fold (f <$> T) → ∃ (g : nat → nat), (∀ i, i ∈ term_fv T → g i ∈ f i) ∧ T' = g <$> T.
 Proof.
-  revert T'. induction T as [x|T1 HT1 T2 HT2|T1 HT1 T2 HT2]=> T' Hlin /=.
+  revert T'. induction T as [x|sp T1 HT1 T2 HT2]=> T' Hlin /=.
   - rewrite elem_of_map. intros [y [-> Hy]]. exists (const y). set_solver.
-  - rewrite sets.elem_of_set_map_2.
-    intros (T1' & T2' & -> & HT1' & HT2').
-    destruct Hlin as [Hfv [Hlin1 Hlin2]].
-    destruct (HT1 _ Hlin1 HT1') as [g1 [Hg1 Hg1']].
-    destruct (HT2 _ Hlin2 HT2') as [g2 [Hg2 Hg2']].
-    exists (λ i, match (decide (i ∈ term_fv T1)) with left _ => g1 i | right _ => g2 i end).
-    split.
-    { intros i. rewrite elem_of_union. intros [Hi1 | Hi2].
-      - rewrite decide_True //. eauto.
-      - rewrite decide_False //.
-        { intros ?. specialize (Hfv i). naive_solver. }
-        by apply Hg2. }
-    f_equiv.
-    { rewrite Hg1'.
-      apply bterm_fmap_ext; auto.
-      intros x Hx. rewrite decide_True //. }
-    { rewrite Hg2'.
-      apply bterm_fmap_ext; auto.
-      intros x Hx. assert (x ∉ term_fv T1) by set_solver.
-      rewrite decide_False //. }
   - rewrite sets.elem_of_set_map_2.
     intros (T1' & T2' & -> & HT1' & HT2').
     destruct Hlin as [Hfv [Hlin1 Hlin2]].
@@ -452,4 +353,4 @@ Qed.
 
 (* XXX: unset the results of loading Equations *)
 Global Obligation Tactic := idtac.
-(* IMPORTANT: make sure that Equations is loadeded *before* this module, otherwise this will be overwritten. *)
+(* XXX IMPORTANT: make sure that Equations is loadeded *before* this module, otherwise this will be overwritten. *)
