theories/seqcalc_height.v
@@ -25,11 +25,11 @@ Module SeqcalcHeight(R : ANALYTIC_STRUCT_EXT).
       Δ1 =? Δ2 →
       fill C Δ1 =? fill C Δ2
   | BE_comma_unit_l Δ :
-      (empty ,, Δ)%B =? Δ
+      (∅ₘ ,, Δ)%B =? Δ
   | BE_comma_comm Δ1 Δ2 :
       (Δ1 ,, Δ2)%B =? (Δ2 ,, Δ1)%B
   | BE_comma_assoc Δ1 Δ2 Δ3 : (Δ1 ,, (Δ2 ,, Δ3))%B =? ((Δ1 ,, Δ2) ,, Δ3)%B
-  | BE_semic_unit_l Δ : (top ;, Δ)%B =? Δ
+  | BE_semic_unit_l Δ : (∅ₐ ;, Δ)%B =? Δ
   | BE_semic_comm Δ1 Δ2  : (Δ1 ;, Δ2)%B =? (Δ2 ;, Δ1)%B
   | BE_semic_assoc Δ1 Δ2 Δ3  : (Δ1 ;, (Δ2 ;, Δ3))%B =? ((Δ1 ;, Δ2) ;, Δ3)%B
   where "Δ =? Γ" := (bunch_equiv Δ%B Γ%B).
@@ -44,7 +44,7 @@ Module SeqcalcHeight(R : ANALYTIC_STRUCT_EXT).
     (Δ ≡ Δ') → (bunch_equiv_h Δ Δ').
   Proof.
     induction 1.
-    all: try by (eapply rtsc_lr; econstructor).
+    all: try by (eapply rtsc_lr; destruct s; econstructor).
     - unfold bunch_equiv_h. reflexivity.
     - by symmetry.
     - etrans; eauto.
@@ -78,84 +78,84 @@ Module SeqcalcHeight(R : ANALYTIC_STRUCT_EXT).
         by rewrite HC2.
     + apply bunch_decomp_complete in heqY.
       inversion heqY; simplify_eq/=.
-      { inversion H3. }
-      apply bunch_decomp_correct in H3.
+      { inversion H4. }
+      apply bunch_decomp_correct in H4.
       exists Π. split; eauto.
       intros X. rewrite fill_app /= left_id //.
     + apply bunch_decomp_complete in heqY.
       inversion heqY; simplify_eq/=.
       * exists (Π ++ [CtxCommaR Δ2]). split.
         { rewrite fill_app/=.
-          apply bunch_decomp_correct in H3.
-          by rewrite H3. }
+          apply bunch_decomp_correct in H4.
+          by rewrite H4. }
         intros Δ. rewrite !fill_app/=.
         by rewrite comm.
       * exists (Π ++ [CtxCommaL Δ1]). split.
         { rewrite fill_app/=.
-          apply bunch_decomp_correct in H3.
-          by rewrite H3. }
+          apply bunch_decomp_correct in H4.
+          by rewrite H4. }
         intros Δ. rewrite !fill_app/=.
         by rewrite comm.
     + apply bunch_decomp_complete in heqY.
       inversion heqY; simplify_eq/=.
       * exists (Π ++ [CtxCommaL Δ2;CtxCommaL Δ3])%B. split.
         { rewrite fill_app/=.
-          apply bunch_decomp_correct in H3.
-          by rewrite H3. }
+          apply bunch_decomp_correct in H4.
+          by rewrite H4. }
         intros Δ. rewrite !fill_app/=.
         by rewrite assoc.
-      * inversion H3; simplify_eq/=.
+      * inversion H4; simplify_eq/=.
         ** exists (Π0 ++ [CtxCommaR Δ1;CtxCommaL Δ3])%B. split.
            { rewrite fill_app/=.
-             apply bunch_decomp_correct in H4.
-               by rewrite H4. }
+             apply bunch_decomp_correct in H5.
+             by rewrite H5. }
            intros Δ. rewrite !fill_app/=.
            by rewrite assoc.
         ** exists (Π0 ++ [CtxCommaR (Δ1,,Δ2)])%B. split.
            { simpl. rewrite fill_app/=.
-             apply bunch_decomp_correct in H4.
-             by rewrite H4. }
+             apply bunch_decomp_correct in H5.
+             by rewrite H5. }
            intros Δ. rewrite !fill_app/=.
            by rewrite assoc.
     + apply bunch_decomp_complete in heqY.
       inversion heqY; simplify_eq/=.
-      { inversion H3. }
-      apply bunch_decomp_correct in H3.
+      { inversion H4. }
+      apply bunch_decomp_correct in H4.
       exists Π. split; eauto.
       intros X. rewrite fill_app /= left_id //.
     + apply bunch_decomp_complete in heqY.
       inversion heqY; simplify_eq/=.
       * exists (Π ++ [CtxSemicR Δ2]). split.
         { rewrite fill_app/=.
-          apply bunch_decomp_correct in H3.
-          by rewrite H3. }
+          apply bunch_decomp_correct in H4.
+          by rewrite H4. }
         intros Δ. rewrite !fill_app/=.
         by rewrite comm.
       * exists (Π ++ [CtxSemicL Δ1]). split.
         { rewrite fill_app/=.
-          apply bunch_decomp_correct in H3.
-          by rewrite H3. }
+          apply bunch_decomp_correct in H4.
+          by rewrite H4. }
         intros Δ. rewrite !fill_app/=.
         by rewrite comm.
     + apply bunch_decomp_complete in heqY.
       inversion heqY; simplify_eq/=.
       * exists (Π ++ [CtxSemicL Δ2;CtxSemicL Δ3])%B. split.
         { rewrite fill_app/=.
-          apply bunch_decomp_correct in H3.
-          by rewrite H3. }
+          apply bunch_decomp_correct in H4.
+          by rewrite H4. }
         intros Δ. rewrite !fill_app/=.
         by rewrite assoc.
-      * inversion H3; simplify_eq/=.
+      * inversion H4; simplify_eq/=.
         ** exists (Π0 ++ [CtxSemicR Δ1;CtxSemicL Δ3])%B. split.
            { rewrite fill_app/=.
-             apply bunch_decomp_correct in H4.
-               by rewrite H4. }
+             apply bunch_decomp_correct in H5.
+             by rewrite H5. }
            intros Δ. rewrite !fill_app/=.
            by rewrite assoc.
         ** exists (Π0 ++ [CtxSemicR (Δ1;,Δ2)])%B. split.
            { simpl. rewrite fill_app/=.
-             apply bunch_decomp_correct in H4.
-             by rewrite H4. }
+             apply bunch_decomp_correct in H5.
+             by rewrite H5. }
            intros Δ. rewrite !fill_app/=.
            by rewrite assoc.
   Qed.
@@ -183,7 +183,7 @@ Module SeqcalcHeight(R : ANALYTIC_STRUCT_EXT).
         assert (Δ1 ≡ Δ2) as ->.
         { by apply bunch_equiv_1. }
         by rewrite HC2.
-    + exists (C' ++ [CtxCommaR empty]). simpl; split.
+    + exists (C' ++ [CtxCommaR ∅ₘ]%B). simpl; split.
       { rewrite fill_app /=. by rewrite heqY. }
       intros X; rewrite fill_app/=.
       by rewrite left_id.
@@ -191,38 +191,38 @@ Module SeqcalcHeight(R : ANALYTIC_STRUCT_EXT).
       inversion heqY; simplify_eq/=.
       * exists (Π ++ [CtxCommaR Δ1]). split.
         { rewrite fill_app/=.
-          apply bunch_decomp_correct in H3.
-          by rewrite H3. }
+          apply bunch_decomp_correct in H4.
+          by rewrite H4. }
         intros Δ. rewrite !fill_app/=.
         by rewrite comm.
       * exists (Π ++ [CtxCommaL Δ2]). split.
         { rewrite fill_app/=.
-          apply bunch_decomp_correct in H3.
-          by rewrite H3. }
+          apply bunch_decomp_correct in H4.
+          by rewrite H4. }
         intros Δ. rewrite !fill_app/=.
         by rewrite comm.
     + apply bunch_decomp_complete in heqY.
       inversion heqY; simplify_eq/=.
-      * inversion H3; simplify_eq/=.
+      * inversion H4; simplify_eq/=.
         ** exists (Π0 ++ [CtxCommaL (Δ2 ,, Δ3)])%B. split.
            { rewrite fill_app/=.
-             apply bunch_decomp_correct in H4.
-               by rewrite H4. }
+             apply bunch_decomp_correct in H5.
+             by rewrite H5. }
            intros Δ. rewrite !fill_app/=.
            by rewrite assoc.
         ** exists (Π0 ++ [CtxCommaL Δ3;CtxCommaR Δ1])%B. split.
            { simpl. rewrite fill_app/=.
-             apply bunch_decomp_correct in H4.
-             by rewrite H4. }
+             apply bunch_decomp_correct in H5.
+             by rewrite H5. }
            intros Δ. rewrite !fill_app/=.
            by rewrite assoc.
       * exists (Π ++ [CtxCommaR Δ2;CtxCommaR Δ1])%B. split.
         { rewrite fill_app/=.
-          apply bunch_decomp_correct in H3.
-            by rewrite H3. }
+          apply bunch_decomp_correct in H4.
+            by rewrite H4. }
            intros Δ. rewrite !fill_app/=.
            by rewrite assoc.
-    + exists (C' ++ [CtxSemicR top]). simpl; split.
+    + exists (C' ++ [CtxSemicR ∅ₐ]%B). simpl; split.
       { rewrite fill_app /=. by rewrite heqY. }
       intros X; rewrite fill_app/=.
       by rewrite left_id.
@@ -230,35 +230,35 @@ Module SeqcalcHeight(R : ANALYTIC_STRUCT_EXT).
       inversion heqY; simplify_eq/=.
       * exists (Π ++ [CtxSemicR Δ1]). split.
         { rewrite fill_app/=.
-          apply bunch_decomp_correct in H3.
-          by rewrite H3. }
+          apply bunch_decomp_correct in H4.
+          by rewrite H4. }
         intros Δ. rewrite !fill_app/=.
         by rewrite comm.
       * exists (Π ++ [CtxSemicL Δ2]). split.
         { rewrite fill_app/=.
-          apply bunch_decomp_correct in H3.
-          by rewrite H3. }
+          apply bunch_decomp_correct in H4.
+          by rewrite H4. }
         intros Δ. rewrite !fill_app/=.
         by rewrite comm.
     + apply bunch_decomp_complete in heqY.
       inversion heqY; simplify_eq/=.
-      * inversion H3; simplify_eq/=.
+      * inversion H4; simplify_eq/=.
         ** exists (Π0 ++ [CtxSemicL (Δ2 ;, Δ3)])%B. split.
            { rewrite fill_app/=.
-             apply bunch_decomp_correct in H4.
-             by rewrite H4. }
+             apply bunch_decomp_correct in H5.
+             by rewrite H5. }
            intros Δ. rewrite !fill_app/=.
            by rewrite assoc.
         ** exists (Π0 ++ [CtxSemicL Δ3;CtxSemicR Δ1])%B. split.
            { simpl. rewrite fill_app/=.
-             apply bunch_decomp_correct in H4.
-             by rewrite H4. }
+             apply bunch_decomp_correct in H5.
+             by rewrite H5. }
            intros Δ. rewrite !fill_app/=.
            by rewrite assoc.
       * exists (Π ++ [CtxSemicR Δ2;CtxSemicR Δ1])%B. split.
         { rewrite fill_app/=.
-          apply bunch_decomp_correct in H3.
-            by rewrite H3. }
+          apply bunch_decomp_correct in H4.
+            by rewrite H4. }
            intros Δ. rewrite !fill_app/=.
            by rewrite assoc.
   Qed.
@@ -302,9 +302,9 @@ Module SeqcalcHeight(R : ANALYTIC_STRUCT_EXT).
     fill Π (bterm_ctx_act T Δs) ⊢ᴮ{S n} ϕ
   (* multiplicatives *)
   | BI_Emp_R :
-      empty ⊢ᴮ{0} EMP
+      ∅ₘ ⊢ᴮ{0} EMP
   | BI_Emp_L C ϕ n :
-      (fill C empty ⊢ᴮ{n} ϕ) →
+      (fill C ∅ₘ ⊢ᴮ{n} ϕ) →
       fill C (frml EMP) ⊢ᴮ{S n} ϕ
   | BI_Sep_R Δ Δ' ϕ ψ n m :
       (Δ ⊢ᴮ{n} ϕ) →
@@ -326,7 +326,7 @@ Module SeqcalcHeight(R : ANALYTIC_STRUCT_EXT).
   | BI_True_R Δ :
       Δ ⊢ᴮ{0} TOP
   | BI_True_L C ϕ n :
-      (fill C top ⊢ᴮ{n} ϕ) →
+      (fill C ∅ₐ ⊢ᴮ{n} ϕ) →
       fill C (frml TOP) ⊢ᴮ{S n} ϕ
   | BI_Conj_R Δ Δ' ϕ ψ n m :
       (Δ ⊢ᴮ{n} ϕ) →
@@ -461,14 +461,15 @@ Module SeqcalcHeight(R : ANALYTIC_STRUCT_EXT).
     - commute_left_rule IHproves2.
   Qed.
 
-  Lemma sep_l_inv' Δ C ϕ ψ χ n :
+  Lemma collapse_l_inv' Δ Π Δ' ϕ χ n :
+    collapse_gr Δ' ϕ →
     (Δ ⊢ᴮ{n} χ) →
-    Δ = fill C (frml (SEP ϕ ψ)) →
-    (fill C (frml ϕ,, frml ψ) ⊢ᴮ{n} χ).
+    Δ = fill Π (frml ϕ) →
+    (fill Π Δ' ⊢ᴮ{n} χ).
   Proof.
-    revert C Δ χ.
-    induction n using lt_wf_ind. rename H into IHproves.
-    intros C Δ χ PROOF Heq. symmetry in Heq. revert Heq.
+    revert Π Δ Δ' ϕ χ.
+    induction n as [n IHproves] using lt_wf_ind.
+    intros Π Δ Δ' ϕ χ Hcoll PROOF Heq. symmetry in Heq. revert Heq.
     inversion PROOF; simplify_eq/= => Heq.
     (* induction H => C' Heq; symmetry in Heq. *)
     - (* raising the pf height *)
@@ -476,7 +477,7 @@ Module SeqcalcHeight(R : ANALYTIC_STRUCT_EXT).
       eapply IHproves; eauto.
     - (* axiom *)
       apply fill_is_frml in Heq. destruct_and!; simplify_eq/=.
-      (* eapply BI_Sep_R; by econstructor. *)
+      inversion Hcoll. by econstructor.
     - (* equivalence of bunches *)
       simplify_eq/=.
       destruct (bunch_equiv_fill _ _ _ H) as [C2 [-> HC2]].
@@ -496,7 +497,7 @@ Module SeqcalcHeight(R : ANALYTIC_STRUCT_EXT).
           by apply bunch_decomp_correct, bunch_decomp_app.
         * rewrite !fill_app/=.
           by apply BI_Weaken.
-      + rename C0 into C'.
+      + rename C into C'.
         destruct H2 as (C0 & C1 & HC0 & HC1 & Hdec0).
         rewrite -HC1.
         apply BI_Weaken.
@@ -507,28 +508,28 @@ Module SeqcalcHeight(R : ANALYTIC_STRUCT_EXT).
       apply bunch_decomp_complete in Heq.
       apply bunch_decomp_ctx in Heq.
       destruct Heq as [H1 | H2]; last first.
-      + rename C0 into C'.
+      + rename C into C'.
         destruct H2 as (C0 & C1 & HC0 & HC1 & Hdec0).
         rewrite -HC1.
         apply BI_Contr.
         rewrite -HC0.
         eapply IHproves; eauto.
         apply bunch_decomp_correct. apply Hdec0.
-      + rename C0 into C'.
+      + rename C into C'.
         destruct H1 as [C0 [HC0 ->]].
         apply bunch_decomp_correct in HC0.
         simplify_eq/=.
-        assert (fill C' (fill C0 (frml ϕ,, frml ψ);, fill C0 (frml (SEP ϕ ψ))) ⊢ᴮ{ n0} χ) as IH1.
+        assert (fill C' (fill C0 Δ';, fill C0 (frml ϕ)) ⊢ᴮ{ n0} χ) as IH1.
         { specialize (IHproves n0 (lt_n_Sn _)).
-          set (C2 := (C0 ++ [CtxSemicL (fill C0 (frml (SEP ϕ ψ)))] ++ C')%B).
-          specialize (IHproves C2 _ _ H).
+          set (C2 := (C0 ++ [CtxSemicL (fill C0 (frml ϕ))] ++ C')%B).
+          specialize (IHproves C2 _ _ _ _ Hcoll H).
           revert IHproves. rewrite /C2 !fill_app /=.
           eauto. }
         rewrite fill_app.
         apply BI_Contr.
-        set (C2 := (C0 ++ [CtxSemicR (fill C0 (frml ϕ,, frml ψ))] ++ C')%B).
-        replace (fill C' (fill C0 (frml ϕ,, frml ψ);, fill C0 (frml ϕ,, frml ψ)))%B
-                   with (fill C2 (frml ϕ,, frml ψ))%B by rewrite fill_app//.
+        set (C2 := (C0 ++ [CtxSemicR (fill C0 Δ')] ++ C')%B).
+        replace (fill C' (fill C0 Δ';, fill C0 Δ'))%B
+                   with (fill C2 Δ')%B by rewrite fill_app//.
         eapply IHproves; eauto.
         rewrite /C2 fill_app//.
     - (* ext *)
@@ -550,44 +551,31 @@ Module SeqcalcHeight(R : ANALYTIC_STRUCT_EXT).
         destruct HC0 as (j & Π₀ & Hjfv & Hj & HC0).
         rewrite fill_app -HC0.
         eapply BI_Simple_Ext; eauto.
-        revert Hj Hjfv IHproves H0.
+        revert Hj Hjfv IHproves H0 Hcoll.
         clear.
-        intros Hj Hjfv IHproves Hpfs.
+        intros Hj Hjfv IHproves Hpfs Hcoll.
         intros Ti HTi. specialize (Hpfs Ti HTi).
-        revert Π Hpfs. clear HTi.
-        induction Ti=>Π Hpfs.
+        revert Π0 Hpfs. clear HTi.
+        induction Ti=>Π0 Hpfs.
         { simpl.
           destruct (decide (j = x)) as [->|?].
           - rewrite functions.fn_lookup_insert.
-            rewrite -fill_app.
+            rewrite -fill_app. simpl in Hpfs.
             eapply IHproves; eauto.
             by rewrite fill_app -Hj.
           - rewrite functions.fn_lookup_insert_ne; auto. }
         { simpl.
-          assert (fill ([CtxCommaL (bterm_ctx_act Ti2 Δs)]++Π) (bterm_ctx_act Ti1 (<[j:=fill Π₀ (frml ϕ,, frml ψ)]> Δs)) ⊢ᴮ{ n0} χ) as HH1.
+          assert (fill ([CtxL sp (bterm_ctx_act Ti2 Δs)]++Π0) (bterm_ctx_act Ti1 (<[j:=fill Π₀ Δ']> Δs)) ⊢ᴮ{ n0} χ) as HH1.
           { eapply IHTi1. rewrite fill_app /=. eauto. }
           rewrite fill_app in HH1.
           simpl in HH1.
           replace
-          (fill Π (bterm_ctx_act Ti1
-             (<[j:=fill Π₀ (frml ϕ,, frml ψ)]> Δs),,bterm_ctx_act Ti2 (<[j:=fill Π₀ (frml ϕ,, frml ψ)]> Δs)))%B
+            (fill Π0 (bbin sp
+                       (bterm_ctx_act Ti1
+             (<[j:=fill Π₀ Δ']> Δs)) (bterm_ctx_act Ti2 (<[j:=fill Π₀ Δ']> Δs))))%B
             with
-          (fill ([CtxCommaR (bterm_ctx_act Ti1 (<[j:=fill Π₀ (frml ϕ,, frml ψ)]> Δs))]++Π)
-                (bterm_ctx_act Ti2 (<[j:=fill Π₀ (frml ϕ,, frml ψ)]> Δs)))%B
-            by rewrite fill_app//.
-          eapply IHTi2.
-          rewrite fill_app/=//. }
-        { simpl.
-          assert (fill ([CtxSemicL (bterm_ctx_act Ti2 Δs)]++Π) (bterm_ctx_act Ti1 (<[j:=fill Π₀ (frml ϕ,, frml ψ)]> Δs)) ⊢ᴮ{ n0} χ) as HH1.
-          { eapply IHTi1. rewrite fill_app /=. eauto. }
-          rewrite fill_app in HH1.
-          simpl in HH1.
-          replace
-          (fill Π (bterm_ctx_act Ti1
-             (<[j:=fill Π₀ (frml ϕ,, frml ψ)]> Δs);,bterm_ctx_act Ti2 (<[j:=fill Π₀ (frml ϕ,, frml ψ)]> Δs)))%B
-            with
-          (fill ([CtxSemicR (bterm_ctx_act Ti1 (<[j:=fill Π₀ (frml ϕ,, frml ψ)]> Δs))]++Π)
-                (bterm_ctx_act Ti2 (<[j:=fill Π₀ (frml ϕ,, frml ψ)]> Δs)))%B
+          (fill ([CtxR sp (bterm_ctx_act Ti1 (<[j:=fill Π₀ Δ']> Δs))]++Π0)
+                (bterm_ctx_act Ti2 (<[j:=fill Π₀ Δ']> Δs)))%B
             by rewrite fill_app//.
           eapply IHTi2.
           rewrite fill_app/=//. }
@@ -601,7 +589,10 @@ Module SeqcalcHeight(R : ANALYTIC_STRUCT_EXT).
       destruct Heq as [H1 | H2].
       + destruct H1 as [C1 [HC0 HC]].
         inversion HC0; simplify_eq/=.
-      + rename C0 into C'.
+        inversion Hcoll; simplify_eq/=.
+        * by apply BI_Emp_L.
+        * by apply BI_Higher.
+      + rename C into C'.
         destruct H2 as (C0 & C1 & HC0 & HC1 & Hdec0).
         rewrite -HC1.
         apply BI_Emp_L.
@@ -625,56 +616,72 @@ Module SeqcalcHeight(R : ANALYTIC_STRUCT_EXT).
       destruct Heq as [H1 | H2].
       + destruct H1 as [C1 [HC0 HC]].
         inversion HC0; simplify_eq/=.
+        inversion Hcoll; simplify_eq/=; eauto.
+        assert (fill C (Δ1,, frml ψ) ⊢ᴮ{ n0} χ) as H1.
+        { replace (fill C (Δ1,, frml ψ))%B
+            with (fill ([CtxCommaL (frml ψ)]++C) Δ1)
+            by rewrite fill_app//.
+          eapply IHproves; eauto. }
+        replace (fill C (Δ1,, Δ2))%B
+          with (fill ([CtxCommaR Δ1]++C) Δ2)
+          by rewrite fill_app//.
+        apply BI_Higher.
+        eapply IHproves; eauto.
+      + rename C into C'.
+        destruct H2 as (C0 & C1 & HC0 & HC1 & Hdec0).
+        rewrite -HC1.
+        apply BI_Sep_L.
+        rewrite -HC0.
+        eapply IHproves; eauto.
+        apply bunch_decomp_correct. apply Hdec0.
+    - (* wand R *)
+      apply BI_Wand_R.
+      replace (fill Π Δ',, frml ϕ0)%B
+        with (fill (Π ++ [CtxCommaL (frml ϕ0)]) Δ')%B
+        by rewrite fill_app//.
+      eapply IHproves; eauto. rewrite -Heq fill_app /= //.
+    - (* wand L *)
+      apply bunch_decomp_complete in Heq.
+      apply bunch_decomp_ctx in Heq.
+      destruct Heq as [H1 | H2].
+      + destruct H1 as [C1 [HC0 HC]].
+        inversion HC0; simplify_eq/=.
+        * rewrite !fill_app/=.
+          eapply BI_Wand_L; eauto.
+          eapply IHproves; eauto; first lia.
+          by apply bunch_decomp_correct.
+        * inversion H6; subst.
+          inversion Hcoll; subst.
+          simpl.
+          eapply BI_Wand_L; eauto.
+      + rename C into C'.
+        destruct H2 as (C0 & C1 & HC0 & HC1 & Hdec0).
+        rewrite -HC1.
+        apply BI_Wand_L; eauto.
+        rewrite -HC0.
+        eapply IHproves; eauto; first lia.
+        apply bunch_decomp_correct. apply Hdec0.
+    - (* bot L *)
+      apply bunch_decomp_complete in Heq.
+      apply bunch_decomp_ctx in Heq.
+      destruct Heq as [H1 | H2].
+      + destruct H1 as [C1 [HC0 HC]].
+        inversion HC0; simplify_eq/=.
+        inversion Hcoll; eauto.
+      + rename C into C'.
+        destruct H2 as (C0 & C1 & HC0 & HC1 & Hdec0).
+        rewrite -HC1.
+        apply BI_False_L.
+    - (* top R *) apply BI_True_R.
+    - (* top L *)
+      apply bunch_decomp_complete in Heq.
+      apply bunch_decomp_ctx in Heq.
+      destruct Heq as [H1 | H2].
+      + destruct H1 as [C1 [HC0 HC]].
+        inversion HC0; simplify_eq/=.
+        inversion Hcoll; subst; eauto.
         by apply BI_Higher.
-      + rename C0 into C'.
-        destruct H2 as (C0 & C1 & HC0 & HC1 & Hdec0).
-        rewrite -HC1.
-        apply BI_Sep_L.
-        rewrite -HC0.
-        eapply IHproves; eauto.
-        apply bunch_decomp_correct. apply Hdec0.
-    - (* wand R *)
-      apply BI_Wand_R.
-      assert ((fill C (frml ϕ,, frml ψ),, frml ϕ0) =
-                   fill (C ++ [CtxCommaL (frml ϕ0)]) (frml ϕ,, frml ψ))%B as ->.
-      { rewrite fill_app//. }
-      eapply IHproves; eauto. rewrite -Heq fill_app /= //.
-    - (* wand L *)
-      apply bunch_decomp_complete in Heq.
-      apply bunch_decomp_ctx in Heq.
-      destruct Heq as [H1 | H2].
-      + destruct H1 as [C1 [HC0 HC]].
-        inversion HC0; simplify_eq/=.
-        * rewrite !fill_app/=.
-          eapply BI_Wand_L; eauto.
-          eapply IHproves; eauto; first lia.
-          by apply bunch_decomp_correct.
-        * exfalso. inversion H5.
-      + rename C0 into C'.
-        destruct H2 as (C0 & C1 & HC0 & HC1 & Hdec0).
-        rewrite -HC1.
-        apply BI_Wand_L; eauto.
-        rewrite -HC0.
-        eapply IHproves; eauto; first lia.
-        apply bunch_decomp_correct. apply Hdec0.
-    - (* bot L *)
-      apply bunch_decomp_complete in Heq.
-      apply bunch_decomp_ctx in Heq.
-      destruct Heq as [H1 | H2].
-      + destruct H1 as [C1 [HC0 HC]].
-        inversion HC0; simplify_eq/=.
-      + rename C0 into C'.
-        destruct H2 as (C0 & C1 & HC0 & HC1 & Hdec0).
-        rewrite -HC1.
-        apply BI_False_L.
-    - (* top R *) apply BI_True_R.
-    - (* top L *)
-      apply bunch_decomp_complete in Heq.
-      apply bunch_decomp_ctx in Heq.
-      destruct Heq as [H1 | H2].
-      + destruct H1 as [C1 [HC0 HC]].
-        inversion HC0; simplify_eq/=.
-      + rename C0 into C'.
+      + rename C into C'.
         destruct H2 as (C0 & C1 & HC0 & HC1 & Hdec0).
         rewrite -HC1.
         apply BI_True_L.
@@ -698,7 +705,18 @@ Module SeqcalcHeight(R : ANALYTIC_STRUCT_EXT).
       destruct Heq as [H1 | H2].
       + destruct H1 as [C1 [HC0 HC]].
         inversion HC0; simplify_eq/=.
-      + rename C0 into C'.
+        inversion Hcoll; simplify_eq/=; eauto.
+        assert (fill C (Δ1;, frml ψ) ⊢ᴮ{ n0} χ) as H1.
+        { replace (fill C (Δ1;, frml ψ))%B
+            with (fill ([CtxSemicL (frml ψ)]++C) Δ1)
+            by rewrite fill_app//.
+          eapply IHproves; eauto. }
+        replace (fill C (Δ1;, Δ2))%B
+          with (fill ([CtxSemicR Δ1]++C) Δ2)
+          by rewrite fill_app//.
+        apply BI_Higher.
+        eapply IHproves; eauto.
+      + rename C into C'.
         destruct H2 as (C0 & C1 & HC0 & HC1 & Hdec0).
         rewrite -HC1.
         apply BI_Conj_L.
@@ -717,6 +735,7 @@ Module SeqcalcHeight(R : ANALYTIC_STRUCT_EXT).
       destruct Heq as [H1 | H2].
       + destruct H1 as [C1 [HC0 HC]].
         inversion HC0; simplify_eq/=.
+        inversion Hcoll; simplify_eq/=; eauto.
       + destruct H2 as (C0 & C1 & HC0 & HC1 & Hdec0).
         rewrite -HC1.
         apply BI_Disj_L.
@@ -728,11 +747,11 @@ Module SeqcalcHeight(R : ANALYTIC_STRUCT_EXT).
           apply bunch_decomp_correct. apply Hdec0.
     - (* impl R *)
       apply BI_Impl_R.
-      assert ((fill C (frml ϕ,, frml ψ);, frml ϕ0) =
-                   fill (C ++ [CtxSemicL (frml ϕ0)]) (frml ϕ,, frml ψ))%B as ->.
-      { rewrite fill_app//. }
+      replace (fill Π Δ';, frml ϕ0)%B
+        with (fill (Π ++ [CtxSemicL (frml ϕ0)]) Δ')%B
+        by rewrite fill_app//.
       eapply IHproves; eauto. rewrite -Heq fill_app /= //.
-    -       apply bunch_decomp_complete in Heq.
+    - apply bunch_decomp_complete in Heq.
       apply bunch_decomp_ctx in Heq.
       destruct Heq as [H1 | H2].
       + destruct H1 as [C1 [HC0 HC]].
@@ -741,876 +760,9 @@ Module SeqcalcHeight(R : ANALYTIC_STRUCT_EXT).
           eapply BI_Impl_L; eauto.
           eapply IHproves; eauto; first lia.
           by apply bunch_decomp_correct.
-        * exfalso. inversion H5.
-      + rename C0 into C'.
-        destruct H2 as (C0 & C1 & HC0 & HC1 & Hdec0).
-        rewrite -HC1.
-        apply BI_Impl_L; eauto.
-        rewrite -HC0.
-        eapply IHproves; eauto; first lia.
-        apply bunch_decomp_correct. apply Hdec0.
-  Qed.
-
-  Lemma conj_l_inv' Δ C ϕ ψ χ n :
-    (Δ ⊢ᴮ{n} χ) →
-    Δ = fill C (frml (CONJ ϕ ψ)) →
-    (fill C (frml ϕ;, frml ψ) ⊢ᴮ{n} χ).
-  Proof.
-    revert C Δ χ.
-    induction n using lt_wf_ind. rename H into IHproves.
-    intros C Δ χ PROOF Heq. symmetry in Heq. revert Heq.
-    inversion PROOF; simplify_eq/= => Heq.
-    (* induction H => C' Heq; symmetry in Heq. *)
-    - (* raising the pf height *)
-      apply BI_Higher.
-      eapply IHproves; eauto.
-    - (* axiom *)
-      apply fill_is_frml in Heq. destruct_and!; simplify_eq/=.
-      (* eapply BI_Sep_R; by econstructor. *)
-    - (* equivalence of bunches *)
-      simplify_eq/=.
-      destruct (bunch_equiv_fill _ _ _ H) as [C2 [-> HC2]].
-      eapply BI_Equiv.
-      { apply HC2. }
-      eapply IHproves; eauto.
-    - (* weakening *)
-      apply bunch_decomp_complete in Heq.
-      apply bunch_decomp_ctx in Heq.
-      destruct Heq as [H1 | H2].
-      + destruct H1 as [C1 [HC0 HC]].
-        inversion HC0; simplify_eq/=.
-        * rewrite !fill_app/=.
-          apply BI_Weaken.
-          rewrite -fill_app.
-          eapply IHproves; eauto.
-          by apply bunch_decomp_correct, bunch_decomp_app.
-        * rewrite !fill_app/=.
-          by apply BI_Weaken.
-      + rename C0 into C'.
-        destruct H2 as (C0 & C1 & HC0 & HC1 & Hdec0).
-        rewrite -HC1.
-        apply BI_Weaken.
-        rewrite -HC0.
-        eapply IHproves; eauto.
-        apply bunch_decomp_correct. apply Hdec0.
-    - (* contraction *)
-      apply bunch_decomp_complete in Heq.
-      apply bunch_decomp_ctx in Heq.
-      destruct Heq as [H1 | H2]; last first.
-      + rename C0 into C'.
-        destruct H2 as (C0 & C1 & HC0 & HC1 & Hdec0).
-        rewrite -HC1.
-        apply BI_Contr.
-        rewrite -HC0.
-        eapply IHproves; eauto.
-        apply bunch_decomp_correct. apply Hdec0.
-      + rename C0 into C'.
-        destruct H1 as [C0 [HC0 ->]].
-        apply bunch_decomp_correct in HC0.
-        simplify_eq/=.
-        assert (fill C' (fill C0 (frml ϕ;, frml ψ);, fill C0 (frml (CONJ ϕ ψ))) ⊢ᴮ{ n0} χ) as IH1.
-        { specialize (IHproves n0 (lt_n_Sn _)).
-          set (C2 := (C0 ++ [CtxSemicL (fill C0 (frml (CONJ ϕ ψ)))] ++ C')%B).
-          specialize (IHproves C2 _ _ H).
-          revert IHproves. rewrite /C2 !fill_app /=.
-          eauto. }
-        rewrite fill_app.
-        apply BI_Contr.
-        set (C2 := (C0 ++ [CtxSemicR (fill C0 (frml ϕ;, frml ψ))] ++ C')%B).
-        replace (fill C' (fill C0 (frml ϕ;, frml ψ);, fill C0 (frml ϕ;, frml ψ)))%B
-                   with (fill C2 (frml ϕ;, frml ψ))%B by rewrite fill_app//.
-        eapply IHproves; eauto.
-        rewrite /C2 fill_app//.
-    - (* ext *)
-      apply bunch_decomp_complete in Heq.
-      apply bunch_decomp_ctx in Heq.
-      destruct Heq as [H1 | H2]; last first.
-      + destruct H2 as (C0 & C1 & HC0 & HC1 & Hdec0).
-        rewrite -HC1.
-        eapply BI_Simple_Ext; eauto.
-        intros Ti Hi.
-        rewrite -HC0.
-        eapply IHproves; eauto.
-        apply bunch_decomp_correct. apply Hdec0.
-      + destruct H1 as [C0 [HC0 ->]].
-        apply bunch_decomp_correct in HC0.
-        simplify_eq/=.
-        apply bterm_ctx_act_decomp in HC0; last first.
-        { by eapply (rules_good (Ts,T)). }
-        destruct HC0 as (j & Π₀ & Hjfv & Hj & HC0).
-        rewrite fill_app -HC0.
-        eapply BI_Simple_Ext; eauto.
-        revert Hj Hjfv IHproves H0.
-        clear.
-        intros Hj Hjfv IHproves Hpfs.
-        intros Ti HTi. specialize (Hpfs Ti HTi).
-        revert Π Hpfs. clear HTi.
-        induction Ti=>Π Hpfs.
-        { simpl.
-          destruct (decide (j = x)) as [->|?].
-          - rewrite functions.fn_lookup_insert.
-            rewrite -fill_app.
-            eapply IHproves; eauto.
-            by rewrite fill_app -Hj.
-          - rewrite functions.fn_lookup_insert_ne; auto. }
-        { simpl.
-          assert (fill ([CtxCommaL (bterm_ctx_act Ti2 Δs)]++Π) (bterm_ctx_act Ti1 (<[j:=fill Π₀ (frml ϕ;, frml ψ)]> Δs)) ⊢ᴮ{ n0} χ) as HH1.
-          { eapply IHTi1. rewrite fill_app /=. eauto. }
-          rewrite fill_app in HH1.
-          simpl in HH1.
-          replace
-          (fill Π (bterm_ctx_act Ti1
-             (<[j:=fill Π₀ (frml ϕ;, frml ψ)]> Δs),,bterm_ctx_act Ti2 (<[j:=fill Π₀ (frml ϕ;, frml ψ)]> Δs)))%B
-            with
-          (fill ([CtxCommaR (bterm_ctx_act Ti1 (<[j:=fill Π₀ (frml ϕ;, frml ψ)]> Δs))]++Π)
-                (bterm_ctx_act Ti2 (<[j:=fill Π₀ (frml ϕ;, frml ψ)]> Δs)))%B
-            by rewrite fill_app//.
-          eapply IHTi2.
-          rewrite fill_app/=//. }
-        { simpl.
-          assert (fill ([CtxSemicL (bterm_ctx_act Ti2 Δs)]++Π) (bterm_ctx_act Ti1 (<[j:=fill Π₀ (frml ϕ;, frml ψ)]> Δs)) ⊢ᴮ{ n0} χ) as HH1.
-          { eapply IHTi1. rewrite fill_app /=. eauto. }
-          rewrite fill_app in HH1.
-          simpl in HH1.
-          replace
-          (fill Π (bterm_ctx_act Ti1
-             (<[j:=fill Π₀ (frml ϕ;, frml ψ)]> Δs);,bterm_ctx_act Ti2 (<[j:=fill Π₀ (frml ϕ;, frml ψ)]> Δs)))%B
-            with
-          (fill ([CtxSemicR (bterm_ctx_act Ti1 (<[j:=fill Π₀ (frml ϕ;, frml ψ)]> Δs))]++Π)
-                (bterm_ctx_act Ti2 (<[j:=fill Π₀ (frml ϕ;, frml ψ)]> Δs)))%B
-            by rewrite fill_app//.
-          eapply IHTi2.
-          rewrite fill_app/=//. }
-    - (* emp R *)
-      exfalso.
-      apply bunch_decomp_complete in Heq.
-      inversion Heq.
-    - (* emp L *)
-      apply bunch_decomp_complete in Heq.
-      apply bunch_decomp_ctx in Heq.
-      destruct Heq as [H1 | H2].
-      + destruct H1 as [C1 [HC0 HC]].
-        inversion HC0; simplify_eq/=.
-      + rename C0 into C'.
-        destruct H2 as (C0 & C1 & HC0 & HC1 & Hdec0).
-        rewrite -HC1.
-        apply BI_Emp_L.
-        rewrite -HC0.
-        eapply IHproves; eauto.
-        apply bunch_decomp_correct. apply Hdec0.
-    - (* sep R *)
-      apply bunch_decomp_complete in Heq.
-      inversion Heq; simplify_eq/=.
-      + rewrite fill_app /=.
-        eapply BI_Sep_R; eauto.
-        eapply IHproves; eauto; first lia.
-        by apply bunch_decomp_correct.
-      + rewrite fill_app /=.
-        eapply BI_Sep_R; eauto.
-        eapply IHproves; eauto; first lia.
-        by apply bunch_decomp_correct.
-    - (* sep L *)
-      apply bunch_decomp_complete in Heq.
-      apply bunch_decomp_ctx in Heq.
-      destruct Heq as [H1 | H2].
-      + destruct H1 as [C1 [HC0 HC]].
-        inversion HC0; simplify_eq/=.
-      + rename C0 into C'.
-        destruct H2 as (C0 & C1 & HC0 & HC1 & Hdec0).
-        rewrite -HC1.
-        apply BI_Sep_L.
-        rewrite -HC0.
-        eapply IHproves; eauto.
-        apply bunch_decomp_correct. apply Hdec0.
-    - (* wand R *)
-      apply BI_Wand_R.
-      assert ((fill C (frml ϕ;, frml ψ),, frml ϕ0) =
-                   fill (C ++ [CtxCommaL (frml ϕ0)]) (frml ϕ;, frml ψ))%B as ->.
-      { rewrite fill_app//. }
-      eapply IHproves; eauto. rewrite -Heq fill_app /= //.
-    - (* wand L *)
-      apply bunch_decomp_complete in Heq.
-      apply bunch_decomp_ctx in Heq.
-      destruct Heq as [H1 | H2].
-      + destruct H1 as [C1 [HC0 HC]].
-        inversion HC0; simplify_eq/=.
-        * rewrite !fill_app/=.
-          eapply BI_Wand_L; eauto.
-          eapply IHproves; eauto; first lia.
-          by apply bunch_decomp_correct.
-        * exfalso. inversion H5.
-      + rename C0 into C'.
-        destruct H2 as (C0 & C1 & HC0 & HC1 & Hdec0).
-        rewrite -HC1.
-        apply BI_Wand_L; eauto.
-        rewrite -HC0.
-        eapply IHproves; eauto; first lia.
-        apply bunch_decomp_correct. apply Hdec0.
-    - (* bot L *)
-      apply bunch_decomp_complete in Heq.
-      apply bunch_decomp_ctx in Heq.
-      destruct Heq as [H1 | H2].
-      + destruct H1 as [C1 [HC0 HC]].
-        inversion HC0; simplify_eq/=.
-      + rename C0 into C'.
-        destruct H2 as (C0 & C1 & HC0 & HC1 & Hdec0).
-        rewrite -HC1.
-        apply BI_False_L.
-    - (* top R *) apply BI_True_R.
-    - (* top L *)
-      apply bunch_decomp_complete in Heq.
-      apply bunch_decomp_ctx in Heq.
-      destruct Heq as [H1 | H2].
-      + destruct H1 as [C1 [HC0 HC]].
-        inversion HC0; simplify_eq/=.
-      + rename C0 into C'.
-        destruct H2 as (C0 & C1 & HC0 & HC1 & Hdec0).
-        rewrite -HC1.
-        apply BI_True_L.
-        rewrite -HC0.
-        eapply IHproves; eauto.
-        apply bunch_decomp_correct. apply Hdec0.
-    - (* conjR *)
-      apply bunch_decomp_complete in Heq.
-      inversion Heq; simplify_eq/=.
-      + rewrite fill_app /=.
-        eapply BI_Conj_R; eauto.
-        eapply IHproves; eauto; first lia.
-        by apply bunch_decomp_correct.
-      + rewrite fill_app /=.
-        eapply BI_Conj_R; eauto.
-        eapply IHproves; eauto; first lia.
-        by apply bunch_decomp_correct.
-    - (* conjL *)
-      apply bunch_decomp_complete in Heq.
-      apply bunch_decomp_ctx in Heq.
-      destruct Heq as [H1 | H2].
-      + destruct H1 as [C1 [HC0 HC]].
-        inversion HC0; simplify_eq/=.
-        by apply BI_Higher.
-      + rename C0 into C'.
-        destruct H2 as (C0 & C1 & HC0 & HC1 & Hdec0).
-        rewrite -HC1.
-        apply BI_Conj_L.
-        rewrite -HC0.
-        eapply IHproves; eauto.
-        apply bunch_decomp_correct. apply Hdec0.
-    - (* disj R 1 *)
-      eapply BI_Disj_R1.
-      eapply IHproves; eauto.
-    - (* disj R 2 *)
-      eapply BI_Disj_R2.
-      eapply IHproves; eauto.
-    - (* disj L *)
-      apply bunch_decomp_complete in Heq.
-      apply bunch_decomp_ctx in Heq.
-      destruct Heq as [H1 | H2].
-      + destruct H1 as [C1 [HC0 HC]].
-        inversion HC0; simplify_eq/=.
-      + destruct H2 as (C0 & C1 & HC0 & HC1 & Hdec0).
-        rewrite -HC1.
-        apply BI_Disj_L.
-        * rewrite -HC0.
-          eapply IHproves; eauto; first lia.
-          apply bunch_decomp_correct. apply Hdec0.
-        * rewrite -HC0.
-          eapply IHproves; eauto; first lia.
-          apply bunch_decomp_correct. apply Hdec0.
-    - (* impl R *)
-      apply BI_Impl_R.
-      assert ((fill C (frml ϕ;, frml ψ);, frml ϕ0) =
-                   fill (C ++ [CtxSemicL (frml ϕ0)]) (frml ϕ;, frml ψ))%B as ->.
-      { rewrite fill_app//. }
-      eapply IHproves; eauto. rewrite -Heq fill_app /= //.
-    -       apply bunch_decomp_complete in Heq.
-      apply bunch_decomp_ctx in Heq.
-      destruct Heq as [H1 | H2].
-      + destruct H1 as [C1 [HC0 HC]].
-        inversion HC0; simplify_eq/=.
-        * rewrite !fill_app/=.
-          eapply BI_Impl_L; eauto.
-          eapply IHproves; eauto; first lia.
-          by apply bunch_decomp_correct.
-        * exfalso. inversion H5.
-      + rename C0 into C'.
-        destruct H2 as (C0 & C1 & HC0 & HC1 & Hdec0).
-        rewrite -HC1.
-        apply BI_Impl_L; eauto.
-        rewrite -HC0.
-        eapply IHproves; eauto; first lia.
-        apply bunch_decomp_correct. apply Hdec0.
-  Qed.
-
-  Lemma top_l_inv' Δ C ϕ ψ χ n :
-    (Δ ⊢ᴮ{n} χ) →
-    Δ = fill C (frml TOP) →
-    (fill C top ⊢ᴮ{n} χ).
-  Proof.
-    revert C Δ χ.
-    induction n using lt_wf_ind. rename H into IHproves.
-    intros C Δ χ PROOF Heq. symmetry in Heq. revert Heq.
-    inversion PROOF; simplify_eq/= => Heq.
-    (* induction H => C' Heq; symmetry in Heq. *)
-    - (* raising the pf height *)
-      apply BI_Higher.
-      eapply IHproves; eauto.
-    - (* axiom *)
-      apply fill_is_frml in Heq. destruct_and!; simplify_eq/=.
-    - (* equivalence of bunches *)
-      simplify_eq/=.
-      destruct (bunch_equiv_fill _ _ _ H) as [C2 [-> HC2]].
-      eapply BI_Equiv.
-      { apply HC2. }
-      eapply IHproves; eauto.
-    - (* weakening *)
-      apply bunch_decomp_complete in Heq.
-      apply bunch_decomp_ctx in Heq.
-      destruct Heq as [H1 | H2].
-      + destruct H1 as [C1 [HC0 HC]].
-        inversion HC0; simplify_eq/=.
-        * rewrite !fill_app/=.
-          apply BI_Weaken.
-          rewrite -fill_app.
-          eapply IHproves; eauto.
-          by apply bunch_decomp_correct, bunch_decomp_app.
-        * rewrite !fill_app/=.
-          by apply BI_Weaken.
-      + rename C0 into C'.
-        destruct H2 as (C0 & C1 & HC0 & HC1 & Hdec0).
-        rewrite -HC1.
-        apply BI_Weaken.
-        rewrite -HC0.
-        eapply IHproves; eauto.
-        apply bunch_decomp_correct. apply Hdec0.
-    - (* contraction *)
-      apply bunch_decomp_complete in Heq.
-      apply bunch_decomp_ctx in Heq.
-      destruct Heq as [H1 | H2]; last first.
-      + rename C0 into C'.
-        destruct H2 as (C0 & C1 & HC0 & HC1 & Hdec0).
-        rewrite -HC1.
-        apply BI_Contr.
-        rewrite -HC0.
-        eapply IHproves; eauto.
-        apply bunch_decomp_correct. apply Hdec0.
-      + rename C0 into C'.
-        destruct H1 as [C0 [HC0 ->]].
-        apply bunch_decomp_correct in HC0.
-        simplify_eq/=.
-        assert (fill C' (fill C0 top;, fill C0 (frml TOP)) ⊢ᴮ{ n0} χ) as IH1.
-        { specialize (IHproves n0 (lt_n_Sn _)).
-          set (C2 := (C0 ++ [CtxSemicL (fill C0 (frml TOP))] ++ C')%B).
-          specialize (IHproves C2 _ _ H).
-          revert IHproves. rewrite /C2 !fill_app /=.
-          eauto. }
-        rewrite fill_app.
-        apply BI_Contr.
-        set (C2 := (C0 ++ [CtxSemicR (fill C0 top)] ++ C')%B).
-        replace (fill C' (fill C0 top;, fill C0 top))%B
-                   with (fill C2 top)%B by rewrite fill_app//.
-        eapply IHproves; eauto.
-        rewrite /C2 fill_app//.
-    - (* ext *)
-      apply bunch_decomp_complete in Heq.
-      apply bunch_decomp_ctx in Heq.
-      destruct Heq as [H1 | H2]; last first.
-      + destruct H2 as (C0 & C1 & HC0 & HC1 & Hdec0).
-        rewrite -HC1.
-        eapply BI_Simple_Ext; eauto.
-        intros Ti Hi.
-        rewrite -HC0.
-        eapply IHproves; eauto.
-        apply bunch_decomp_correct. apply Hdec0.
-      + destruct H1 as [C0 [HC0 ->]].
-        apply bunch_decomp_correct in HC0.
-        simplify_eq/=.
-        apply bterm_ctx_act_decomp in HC0; last first.
-        { by eapply (rules_good (Ts, T)). }
-        destruct HC0 as (j & Π₀ & Hjfv & Hj & HC0).
-        rewrite fill_app -HC0.
-        eapply BI_Simple_Ext; eauto.
-        revert Hj Hjfv IHproves H0.
-        clear.
-        intros Hj Hjfv IHproves Hpfs.
-        intros Ti HTi. specialize (Hpfs Ti HTi).
-        revert Π Hpfs. clear HTi.
-        induction Ti=>Π Hpfs.
-        { simpl.
-          destruct (decide (j = x)) as [->|?].
-          - rewrite functions.fn_lookup_insert.
-            rewrite -fill_app.
-            eapply IHproves; eauto.
-            by rewrite fill_app -Hj.
-          - rewrite functions.fn_lookup_insert_ne; auto. }
-        { simpl.
-          assert (fill ([CtxCommaL (bterm_ctx_act Ti2 Δs)]++Π) (bterm_ctx_act Ti1 (<[j:=fill Π₀ top]> Δs)) ⊢ᴮ{ n0} χ) as HH1.
-          { eapply IHTi1. rewrite fill_app /=. eauto. }
-          rewrite fill_app in HH1.
-          simpl in HH1.
-          replace
-          (fill Π (bterm_ctx_act Ti1
-             (<[j:=fill Π₀ top]> Δs),,bterm_ctx_act Ti2 (<[j:=fill Π₀ top]> Δs)))%B
-            with
-          (fill ([CtxCommaR (bterm_ctx_act Ti1 (<[j:=fill Π₀ top]> Δs))]++Π)
-                (bterm_ctx_act Ti2 (<[j:=fill Π₀ top]> Δs)))%B
-            by rewrite fill_app//.
-          eapply IHTi2.
-          rewrite fill_app/=//. }
-        { simpl.
-          assert (fill ([CtxSemicL (bterm_ctx_act Ti2 Δs)]++Π) (bterm_ctx_act Ti1 (<[j:=fill Π₀ top]> Δs)) ⊢ᴮ{ n0} χ) as HH1.
-          { eapply IHTi1. rewrite fill_app /=. eauto. }
-          rewrite fill_app in HH1.
-          simpl in HH1.
-          replace
-          (fill Π (bterm_ctx_act Ti1
-             (<[j:=fill Π₀ top]> Δs);,bterm_ctx_act Ti2 (<[j:=fill Π₀ top]> Δs)))%B
-            with
-          (fill ([CtxSemicR (bterm_ctx_act Ti1 (<[j:=fill Π₀ top]> Δs))]++Π)
-                (bterm_ctx_act Ti2 (<[j:=fill Π₀ top]> Δs)))%B
-            by rewrite fill_app//.
-          eapply IHTi2.
-          rewrite fill_app/=//. }
-    - (* emp R *)
-      exfalso.
-      apply bunch_decomp_complete in Heq.
-      inversion Heq.
-    - (* emp L *)
-      apply bunch_decomp_complete in Heq.
-      apply bunch_decomp_ctx in Heq.
-      destruct Heq as [H1 | H2].
-      + destruct H1 as [C1 [HC0 HC]].
-        inversion HC0; simplify_eq/=.
-      + rename C0 into C'.
-        destruct H2 as (C0 & C1 & HC0 & HC1 & Hdec0).
-        rewrite -HC1.
-        apply BI_Emp_L.
-        rewrite -HC0.
-        eapply IHproves; eauto.
-        apply bunch_decomp_correct. apply Hdec0.
-    - (* sep R *)
-      apply bunch_decomp_complete in Heq.
-      inversion Heq; simplify_eq/=.
-      + rewrite fill_app /=.
-        eapply BI_Sep_R; eauto.
-        eapply IHproves; eauto; first lia.
-        by apply bunch_decomp_correct.
-      + rewrite fill_app /=.
-        eapply BI_Sep_R; eauto.
-        eapply IHproves; eauto; first lia.
-        by apply bunch_decomp_correct.
-    - (* sep L *)
-      apply bunch_decomp_complete in Heq.
-      apply bunch_decomp_ctx in Heq.
-      destruct Heq as [H1 | H2].
-      + destruct H1 as [C1 [HC0 HC]].
-        inversion HC0; simplify_eq/=.
-      + rename C0 into C'.
-        destruct H2 as (C0 & C1 & HC0 & HC1 & Hdec0).
-        rewrite -HC1.
-        apply BI_Sep_L.
-        rewrite -HC0.
-        eapply IHproves; eauto.
-        apply bunch_decomp_correct. apply Hdec0.
-    - (* wand R *)
-      apply BI_Wand_R.
-      assert ((fill C top,, frml ϕ0) =
-                   fill (C ++ [CtxCommaL (frml ϕ0)]) top)%B as ->.
-      { rewrite fill_app//. }
-      eapply IHproves; eauto. rewrite -Heq fill_app /= //.
-    - (* wand L *)
-      apply bunch_decomp_complete in Heq.
-      apply bunch_decomp_ctx in Heq.
-      destruct Heq as [H1 | H2].
-      + destruct H1 as [C1 [HC0 HC]].
-        inversion HC0; simplify_eq/=.
-        * rewrite !fill_app/=.
-          eapply BI_Wand_L; eauto.
-          eapply IHproves; eauto; first lia.
-          by apply bunch_decomp_correct.
-        * exfalso. inversion H5.
-      + rename C0 into C'.
-        destruct H2 as (C0 & C1 & HC0 & HC1 & Hdec0).
-        rewrite -HC1.
-        apply BI_Wand_L; eauto.
-        rewrite -HC0.
-        eapply IHproves; eauto; first lia.
-        apply bunch_decomp_correct. apply Hdec0.
-    - (* bot L *)
-      apply bunch_decomp_complete in Heq.
-      apply bunch_decomp_ctx in Heq.
-      destruct Heq as [H1 | H2].
-      + destruct H1 as [C1 [HC0 HC]].
-        inversion HC0; simplify_eq/=.
-      + rename C0 into C'.
-        destruct H2 as (C0 & C1 & HC0 & HC1 & Hdec0).
-        rewrite -HC1.
-        apply BI_False_L.
-    - (* top R *) apply BI_True_R.
-    - (* top L *)
-      apply bunch_decomp_complete in Heq.
-      apply bunch_decomp_ctx in Heq.
-      destruct Heq as [H1 | H2].
-      + destruct H1 as [C1 [HC0 HC]].
-        inversion HC0; simplify_eq/=.
-        by eapply BI_Higher.
-      + rename C0 into C'.
-        destruct H2 as (C0 & C1 & HC0 & HC1 & Hdec0).
-        rewrite -HC1.
-        apply BI_True_L.
-        rewrite -HC0.
-        eapply IHproves; eauto.
-        apply bunch_decomp_correct. apply Hdec0.
-    - (* conjR *)
-      apply bunch_decomp_complete in Heq.
-      inversion Heq; simplify_eq/=.
-      + rewrite fill_app /=.
-        eapply BI_Conj_R; eauto.
-        eapply IHproves; eauto; first lia.
-        by apply bunch_decomp_correct.
-      + rewrite fill_app /=.
-        eapply BI_Conj_R; eauto.
-        eapply IHproves; eauto; first lia.
-        by apply bunch_decomp_correct.
-    - (* conjL *)
-      apply bunch_decomp_complete in Heq.
-      apply bunch_decomp_ctx in Heq.
-      destruct Heq as [H1 | H2].
-      + destruct H1 as [C1 [HC0 HC]].
-        inversion HC0; simplify_eq/=.
-      + rename C0 into C'.
-        destruct H2 as (C0 & C1 & HC0 & HC1 & Hdec0).
-        rewrite -HC1.
-        apply BI_Conj_L.
-        rewrite -HC0.
-        eapply IHproves; eauto.
-        apply bunch_decomp_correct. apply Hdec0.
-    - (* disj R 1 *)
-      eapply BI_Disj_R1.
-      eapply IHproves; eauto.
-    - (* disj R 2 *)
-      eapply BI_Disj_R2.
-      eapply IHproves; eauto.
-    - (* disj L *)
-      apply bunch_decomp_complete in Heq.
-      apply bunch_decomp_ctx in Heq.
-      destruct Heq as [H1 | H2].
-      + destruct H1 as [C1 [HC0 HC]].
-        inversion HC0; simplify_eq/=.
-      + destruct H2 as (C0 & C1 & HC0 & HC1 & Hdec0).
-        rewrite -HC1.
-        apply BI_Disj_L.
-        * rewrite -HC0.
-          eapply IHproves; eauto; first lia.
-          apply bunch_decomp_correct. apply Hdec0.
-        * rewrite -HC0.
-          eapply IHproves; eauto; first lia.
-          apply bunch_decomp_correct. apply Hdec0.
-    - (* impl R *)
-      apply BI_Impl_R.
-      assert ((fill C top;, frml ϕ0) =
-                   fill (C ++ [CtxSemicL (frml ϕ0)]) top)%B as ->.
-      { rewrite fill_app//. }
-      eapply IHproves; eauto. rewrite -Heq fill_app /= //.
-    -       apply bunch_decomp_complete in Heq.
-      apply bunch_decomp_ctx in Heq.
-      destruct Heq as [H1 | H2].
-      + destruct H1 as [C1 [HC0 HC]].
-        inversion HC0; simplify_eq/=.
-        * rewrite !fill_app/=.
-          eapply BI_Impl_L; eauto.
-          eapply IHproves; eauto; first lia.
-          by apply bunch_decomp_correct.
-        * exfalso. inversion H5.
-      + rename C0 into C'.
-        destruct H2 as (C0 & C1 & HC0 & HC1 & Hdec0).
-        rewrite -HC1.
-        apply BI_Impl_L; eauto.
-        rewrite -HC0.
-        eapply IHproves; eauto; first lia.
-        apply bunch_decomp_correct. apply Hdec0.
-  Qed.
-
-  Lemma emp_l_inv' Δ C ϕ ψ χ n :
-    (Δ ⊢ᴮ{n} χ) →
-    Δ = fill C (frml EMP) →
-    (fill C empty ⊢ᴮ{n} χ).
-  Proof.
-    revert C Δ χ.
-    induction n using lt_wf_ind. rename H into IHproves.
-    intros C Δ χ PROOF Heq. symmetry in Heq. revert Heq.
-    inversion PROOF; simplify_eq/= => Heq.
-    (* induction H => C' Heq; symmetry in Heq. *)
-    - (* raising the pf height *)
-      apply BI_Higher.
-      eapply IHproves; eauto.
-    - (* axiom *)
-      apply fill_is_frml in Heq. destruct_and!; simplify_eq/=.
-    - (* equivalence of bunches *)
-      simplify_eq/=.
-      destruct (bunch_equiv_fill _ _ _ H) as [C2 [-> HC2]].
-      eapply BI_Equiv.
-      { apply HC2. }
-      eapply IHproves; eauto.
-    - (* weakening *)
-      apply bunch_decomp_complete in Heq.
-      apply bunch_decomp_ctx in Heq.
-      destruct Heq as [H1 | H2].
-      + destruct H1 as [C1 [HC0 HC]].
-        inversion HC0; simplify_eq/=.
-        * rewrite !fill_app/=.
-          apply BI_Weaken.
-          rewrite -fill_app.
-          eapply IHproves; eauto.
-          by apply bunch_decomp_correct, bunch_decomp_app.
-        * rewrite !fill_app/=.
-          by apply BI_Weaken.
-      + rename C0 into C'.
-        destruct H2 as (C0 & C1 & HC0 & HC1 & Hdec0).
-        rewrite -HC1.
-        apply BI_Weaken.
-        rewrite -HC0.
-        eapply IHproves; eauto.
-        apply bunch_decomp_correct. apply Hdec0.
-    - (* contraction *)
-      apply bunch_decomp_complete in Heq.
-      apply bunch_decomp_ctx in Heq.
-      destruct Heq as [H1 | H2]; last first.
-      + rename C0 into C'.
-        destruct H2 as (C0 & C1 & HC0 & HC1 & Hdec0).
-        rewrite -HC1.
-        apply BI_Contr.
-        rewrite -HC0.
-        eapply IHproves; eauto.
-        apply bunch_decomp_correct. apply Hdec0.
-      + rename C0 into C'.
-        destruct H1 as [C0 [HC0 ->]].
-        apply bunch_decomp_correct in HC0.
-        simplify_eq/=.
-        assert (fill C' (fill C0 empty;, fill C0 (frml EMP)) ⊢ᴮ{ n0} χ) as IH1.
-        { specialize (IHproves n0 (lt_n_Sn _)).
-          set (C2 := (C0 ++ [CtxSemicL (fill C0 (frml EMP))] ++ C')%B).
-          specialize (IHproves C2 _ _ H).
-          revert IHproves. rewrite /C2 !fill_app /=.
-          eauto. }
-        rewrite fill_app.
-        apply BI_Contr.
-        set (C2 := (C0 ++ [CtxSemicR (fill C0 empty)] ++ C')%B).
-        replace (fill C' (fill C0 empty;, fill C0 empty))%B
-                   with (fill C2 empty)%B by rewrite fill_app//.
-        eapply IHproves; eauto.
-        rewrite /C2 fill_app//.
-    - (* ext *)
-      apply bunch_decomp_complete in Heq.
-      apply bunch_decomp_ctx in Heq.
-      destruct Heq as [H1 | H2]; last first.
-      + destruct H2 as (C0 & C1 & HC0 & HC1 & Hdec0).
-        rewrite -HC1.
-        eapply BI_Simple_Ext; eauto.
-        intros Ti Hi.
-        rewrite -HC0.
-        eapply IHproves; eauto.
-        apply bunch_decomp_correct. apply Hdec0.
-      + destruct H1 as [C0 [HC0 ->]].
-        apply bunch_decomp_correct in HC0.
-        simplify_eq/=.
-        apply bterm_ctx_act_decomp in HC0; last first.
-        { by eapply (rules_good (Ts,T)). }
-        destruct HC0 as (j & Π₀ & Hjfv & Hj & HC0).
-        rewrite fill_app -HC0.
-        eapply BI_Simple_Ext; eauto.
-        revert Hj Hjfv IHproves H0.
-        clear.
-        intros Hj Hjfv IHproves Hpfs.
-        intros Ti HTi. specialize (Hpfs Ti HTi).
-        revert Π Hpfs. clear HTi.
-        induction Ti=>Π Hpfs.
-        { simpl.
-          destruct (decide (j = x)) as [->|?].
-          - rewrite functions.fn_lookup_insert.
-            rewrite -fill_app.
-            eapply IHproves; eauto.
-            by rewrite fill_app -Hj.
-          - rewrite functions.fn_lookup_insert_ne; auto. }
-        { simpl.
-          assert (fill ([CtxCommaL (bterm_ctx_act Ti2 Δs)]++Π) (bterm_ctx_act Ti1 (<[j:=fill Π₀ empty]> Δs)) ⊢ᴮ{ n0} χ) as HH1.
-          { eapply IHTi1. rewrite fill_app /=. eauto. }
-          rewrite fill_app in HH1.
-          simpl in HH1.
-          replace
-          (fill Π (bterm_ctx_act Ti1
-             (<[j:=fill Π₀ empty]> Δs),,bterm_ctx_act Ti2 (<[j:=fill Π₀ empty]> Δs)))%B
-            with
-          (fill ([CtxCommaR (bterm_ctx_act Ti1 (<[j:=fill Π₀ empty]> Δs))]++Π)
-                (bterm_ctx_act Ti2 (<[j:=fill Π₀ empty]> Δs)))%B
-            by rewrite fill_app//.
-          eapply IHTi2.
-          rewrite fill_app/=//. }
-        { simpl.
-          assert (fill ([CtxSemicL (bterm_ctx_act Ti2 Δs)]++Π) (bterm_ctx_act Ti1 (<[j:=fill Π₀ empty]> Δs)) ⊢ᴮ{ n0} χ) as HH1.
-          { eapply IHTi1. rewrite fill_app /=. eauto. }
-          rewrite fill_app in HH1.
-          simpl in HH1.
-          replace
-          (fill Π (bterm_ctx_act Ti1
-             (<[j:=fill Π₀ empty]> Δs);,bterm_ctx_act Ti2 (<[j:=fill Π₀ empty]> Δs)))%B
-            with
-          (fill ([CtxSemicR (bterm_ctx_act Ti1 (<[j:=fill Π₀ empty]> Δs))]++Π)
-                (bterm_ctx_act Ti2 (<[j:=fill Π₀ empty]> Δs)))%B
-            by rewrite fill_app//.
-          eapply IHTi2.
-          rewrite fill_app/=//. }
-    - (* emp R *)
-      exfalso.
-      apply bunch_decomp_complete in Heq.
-      inversion Heq.
-    - (* emp L *)
-      apply bunch_decomp_complete in Heq.
-      apply bunch_decomp_ctx in Heq.
-      destruct Heq as [H1 | H2].
-      + destruct H1 as [C1 [HC0 HC]].
-        inversion HC0; simplify_eq/=.
-        by eapply BI_Higher.
-      + rename C0 into C'.
-        destruct H2 as (C0 & C1 & HC0 & HC1 & Hdec0).
-        rewrite -HC1.
-        apply BI_Emp_L.
-        rewrite -HC0.
-        eapply IHproves; eauto.
-        apply bunch_decomp_correct. apply Hdec0.
-    - (* sep R *)
-      apply bunch_decomp_complete in Heq.
-      inversion Heq; simplify_eq/=.
-      + rewrite fill_app /=.
-        eapply BI_Sep_R; eauto.
-        eapply IHproves; eauto; first lia.
-        by apply bunch_decomp_correct.
-      + rewrite fill_app /=.
-        eapply BI_Sep_R; eauto.
-        eapply IHproves; eauto; first lia.
-        by apply bunch_decomp_correct.
-    - (* sep L *)
-      apply bunch_decomp_complete in Heq.
-      apply bunch_decomp_ctx in Heq.
-      destruct Heq as [H1 | H2].
-      + destruct H1 as [C1 [HC0 HC]].
-        inversion HC0; simplify_eq/=.
-      + rename C0 into C'.
-        destruct H2 as (C0 & C1 & HC0 & HC1 & Hdec0).
-        rewrite -HC1.
-        apply BI_Sep_L.
-        rewrite -HC0.
-        eapply IHproves; eauto.
-        apply bunch_decomp_correct. apply Hdec0.
-    - (* wand R *)
-      apply BI_Wand_R.
-      assert ((fill C empty,, frml ϕ0) =
-                   fill (C ++ [CtxCommaL (frml ϕ0)]) empty)%B as ->.
-      { rewrite fill_app//. }
-      eapply IHproves; eauto. rewrite -Heq fill_app /= //.
-    - (* wand L *)
-      apply bunch_decomp_complete in Heq.
-      apply bunch_decomp_ctx in Heq.
-      destruct Heq as [H1 | H2].
-      + destruct H1 as [C1 [HC0 HC]].
-        inversion HC0; simplify_eq/=.
-        * rewrite !fill_app/=.
-          eapply BI_Wand_L; eauto.
-          eapply IHproves; eauto; first lia.
-          by apply bunch_decomp_correct.
-        * exfalso. inversion H5.
-      + rename C0 into C'.
-        destruct H2 as (C0 & C1 & HC0 & HC1 & Hdec0).
-        rewrite -HC1.
-        apply BI_Wand_L; eauto.
-        rewrite -HC0.
-        eapply IHproves; eauto; first lia.
-        apply bunch_decomp_correct. apply Hdec0.
-    - (* bot L *)
-      apply bunch_decomp_complete in Heq.
-      apply bunch_decomp_ctx in Heq.
-      destruct Heq as [H1 | H2].
-      + destruct H1 as [C1 [HC0 HC]].
-        inversion HC0; simplify_eq/=.
-      + rename C0 into C'.
-        destruct H2 as (C0 & C1 & HC0 & HC1 & Hdec0).
-        rewrite -HC1.
-        apply BI_False_L.
-    - (* true R *) apply BI_True_R.
-    - (* true L *)
-      apply bunch_decomp_complete in Heq.
-      apply bunch_decomp_ctx in Heq.
-      destruct Heq as [H1 | H2].
-      + destruct H1 as [C1 [HC0 HC]].
-        inversion HC0; simplify_eq/=.
-      + rename C0 into C'.
-        destruct H2 as (C0 & C1 & HC0 & HC1 & Hdec0).
-        rewrite -HC1.
-        apply BI_True_L.
-        rewrite -HC0.
-        eapply IHproves; eauto.
-        apply bunch_decomp_correct. apply Hdec0.
-    - (* conjR *)
-      apply bunch_decomp_complete in Heq.
-      inversion Heq; simplify_eq/=.
-      + rewrite fill_app /=.
-        eapply BI_Conj_R; eauto.
-        eapply IHproves; eauto; first lia.
-        by apply bunch_decomp_correct.
-      + rewrite fill_app /=.
-        eapply BI_Conj_R; eauto.
-        eapply IHproves; eauto; first lia.
-        by apply bunch_decomp_correct.
-    - (* conjL *)
-      apply bunch_decomp_complete in Heq.
-      apply bunch_decomp_ctx in Heq.
-      destruct Heq as [H1 | H2].
-      + destruct H1 as [C1 [HC0 HC]].
-        inversion HC0; simplify_eq/=.
-      + rename C0 into C'.
-        destruct H2 as (C0 & C1 & HC0 & HC1 & Hdec0).
-        rewrite -HC1.
-        apply BI_Conj_L.
-        rewrite -HC0.
-        eapply IHproves; eauto.
-        apply bunch_decomp_correct. apply Hdec0.
-    - (* disj R 1 *)
-      eapply BI_Disj_R1.
-      eapply IHproves; eauto.
-    - (* disj R 2 *)
-      eapply BI_Disj_R2.
-      eapply IHproves; eauto.
-    - (* disj L *)
-      apply bunch_decomp_complete in Heq.
-      apply bunch_decomp_ctx in Heq.
-      destruct Heq as [H1 | H2].
-      + destruct H1 as [C1 [HC0 HC]].
-        inversion HC0; simplify_eq/=.
-      + destruct H2 as (C0 & C1 & HC0 & HC1 & Hdec0).
-        rewrite -HC1.
-        apply BI_Disj_L.
-        * rewrite -HC0.
-          eapply IHproves; eauto; first lia.
-          apply bunch_decomp_correct. apply Hdec0.
-        * rewrite -HC0.
-          eapply IHproves; eauto; first lia.
-          apply bunch_decomp_correct. apply Hdec0.
-    - (* impl R *)
-      apply BI_Impl_R.
-      assert ((fill C empty;, frml ϕ0) =
-                   fill (C ++ [CtxSemicL (frml ϕ0)]) empty)%B as ->.
-      { rewrite fill_app//. }
-      eapply IHproves; eauto. rewrite -Heq fill_app /= //.
-    -       apply bunch_decomp_complete in Heq.
-      apply bunch_decomp_ctx in Heq.
-      destruct Heq as [H1 | H2].
-      + destruct H1 as [C1 [HC0 HC]].
-        inversion HC0; simplify_eq/=.
-        * rewrite !fill_app/=.
-          eapply BI_Impl_L; eauto.
-          eapply IHproves; eauto; first lia.
-          by apply bunch_decomp_correct.
-        * exfalso. inversion H5.
-      + rename C0 into C'.
+        * inversion H6; subst.
+          inversion Hcoll; simplify_eq/=; eauto.
+      + rename C into C'.
         destruct H2 as (C0 & C1 & HC0 & HC1 & Hdec0).
         rewrite -HC1.
         apply BI_Impl_L; eauto.
@@ -1642,7 +794,8 @@ Module SeqcalcHeight(R : ANALYTIC_STRUCT_EXT).
   Proof.
     intros [n H]%proves_provesN.
     eapply provesN_proves.
-    eapply sep_l_inv'; eauto.
+    eapply collapse_l_inv'; eauto.
+    by repeat constructor.
   Qed.
   Lemma conj_l_inv C ϕ ψ χ :
     (fill C (frml (CONJ ϕ ψ)) ⊢ᴮ χ) →
@@ -1650,34 +803,16 @@ Module SeqcalcHeight(R : ANALYTIC_STRUCT_EXT).
   Proof.
     intros [n H]%proves_provesN.
     eapply provesN_proves.
-    eapply conj_l_inv'; eauto.
+    eapply collapse_l_inv'; eauto.
+    by repeat constructor.
   Qed.
   Lemma collapse_l_inv C Δ ϕ :
     (fill C (frml (collapse Δ)) ⊢ᴮ ϕ) →
     (fill C Δ ⊢ᴮ ϕ).
   Proof.
-    revert C. induction Δ; simpl; first done.
-    - intros C [n H]%proves_provesN.
-      eapply provesN_proves.
-      eapply top_l_inv'; eauto.
-    - intros C [n H]%proves_provesN.
-      eapply provesN_proves.
-      eapply emp_l_inv'; eauto.
-    - intros C H1.
-      replace (fill C (Δ1,, Δ2))%B
-        with (fill (CtxCommaR Δ1::C) Δ2) by reflexivity.
-      apply IHΔ2. simpl.
-      replace (fill C (Δ1,, frml (collapse Δ2)))%B
-        with (fill (CtxCommaL (frml (collapse Δ2))::C) Δ1) by reflexivity.
-      apply IHΔ1. simpl.
-      by apply sep_l_inv.
-    - intros C H1.
-      replace (fill C (Δ1;, Δ2))%B
-        with (fill (CtxSemicR Δ1::C) Δ2) by reflexivity.
-      apply IHΔ2. simpl.
-      replace (fill C (Δ1;, frml (collapse Δ2)))%B
-        with (fill (CtxSemicL (frml (collapse Δ2))::C) Δ1) by reflexivity.
-      apply IHΔ1. simpl.
-      by apply conj_l_inv.
+    intros [n H]%proves_provesN.
+    eapply provesN_proves.
+    eapply collapse_l_inv'; eauto.
+    apply collapse_gr_sound.
   Qed.
 End SeqcalcHeight.
